Advances in optimizations

ocaml_interface/checker.mli
@@ -1,7 +1,4 @@
 
-type unit0 =
-| Tt
-
 val xorb : bool -> bool -> bool
 
 val negb : bool -> bool
@@ -9,10 +6,6 @@ val negb : bool -> bool
 type nat =
 | O
 | S of nat
-
-type 'a option =
-| Some of 'a
-| None
 
 val fst : ('a1 * 'a2) -> 'a1
 
@@ -260,7 +253,7 @@ module EVM_Def :
 
 module Concrete :
  sig
-  type oper_label =
+  type stack_op_instr =
   | ADD
   | MUL
   | NOT
@@ -320,14 +313,15 @@ module Concrete :
   | POP
   | DUP of nat
   | SWAP of nat
-  | Opcode of oper_label
+  | Opcode of stack_op_instr
 
   type block = instr list
 
-  type operator =
-  | Op of bool * nat * (EVM_Def.coq_EVMWord list -> EVM_Def.coq_EVMWord option)
+  type stack_operation =
+  | StackOp of bool * nat
+     * (EVM_Def.coq_EVMWord list -> EVM_Def.coq_EVMWord option)
 
-  val eq_oper_label : oper_label -> oper_label -> bool
+  val eq_stack_op_instr : stack_op_instr -> stack_op_instr -> bool
 
   val evm_add : EVM_Def.coq_EVMWord list -> EVM_Def.coq_EVMWord option
 
@@ -369,46 +363,48 @@ module Concrete :
 
   type ('k, 'v) map = 'k -> 'v option
 
-  val empty_imap : (oper_label, 'a1) map
+  val empty_imap : (stack_op_instr, 'a1) map
 
-  val updatei : (oper_label, 'a1) map -> oper_label -> 'a1 -> oper_label -> 'a1 option
+  val updatei :
+    (stack_op_instr, 'a1) map -> stack_op_instr -> 'a1 -> stack_op_instr ->
+    'a1 option
 
-  type opm = (oper_label, operator) map
+  type stack_op_map = (stack_op_instr, stack_operation) map
 
-  val fully_defined : oper_label list
+  val fully_defined : stack_op_instr list
 
-  val is_fully_defined : oper_label -> bool
+  val is_fully_defined : stack_op_instr -> bool
 
-  val opmap : opm
+  val evm_stack_opm : stack_op_map
  end
 
 module Abstract :
  sig
-  type asfs_stack_val =
+  type sstack_val =
   | Val of EVM_Def.coq_EVMWord
   | InStackVar of nat
   | FreshVar of nat
 
-  type asfs_map_val =
-  | ASFSBasicVal of asfs_stack_val
-  | ASFSOp of Concrete.oper_label * asfs_stack_val list
+  type smap_val =
+  | SymBasicVal of sstack_val
+  | SymOp of Concrete.stack_op_instr * sstack_val list
 
   type stack_expr =
   | UVal of EVM_Def.coq_EVMWord
   | UInStackVar of nat
-  | UOp of Concrete.oper_label * stack_expr list
+  | UOp of Concrete.stack_op_instr * stack_expr list
 
-  type asfs_stack = asfs_stack_val list
+  type sstack = sstack_val list
 
-  type asfs_map = (nat * asfs_map_val) list
+  type smap = (nat * smap_val) list
 
-  type asfs =
-  | ASFSc of nat * nat * asfs_stack * asfs_map
+  type sstate =
+  | SymState of nat * nat * sstack * smap
  end
 
 module Optimizations :
  sig
-  type optimization = Abstract.asfs -> Abstract.asfs * bool
+  type optim = Abstract.sstate -> Abstract.sstate * bool
  end
 
 val firstn_e : nat -> 'a1 list -> 'a1 list option
@@ -425,168 +421,208 @@ module SFS :
 
   val swap : nat -> 'a1 list -> 'a1 list option
 
-  val get_maxid_asfs : Abstract.asfs -> nat
+  val get_maxid_asfs : Abstract.sstate -> nat
 
-  val get_stack_asfs : Abstract.asfs -> Abstract.asfs_stack
+  val get_stack_asfs : Abstract.sstate -> Abstract.sstack
 
-  val get_map_asfs : Abstract.asfs -> Abstract.asfs_map
+  val get_map_asfs : Abstract.sstate -> Abstract.smap
 
-  val set_maxid_asfs : Abstract.asfs -> nat -> Abstract.asfs
+  val set_maxid_asfs : Abstract.sstate -> nat -> Abstract.sstate
 
-  val set_stack_asfs : Abstract.asfs -> Abstract.asfs_stack -> Abstract.asfs
+  val set_stack_asfs : Abstract.sstate -> Abstract.sstack -> Abstract.sstate
 
-  val set_map_asfs : Abstract.asfs -> Abstract.asfs_map -> Abstract.asfs
+  val set_map_asfs : Abstract.sstate -> Abstract.smap -> Abstract.sstate
 
-  val gen_initial_stack : nat -> Abstract.asfs_stack_val list
+  val gen_initial_stack : nat -> Abstract.sstack
 
-  val empty_asfs : nat -> Abstract.asfs
+  val empty_asfs : nat -> Abstract.sstate
 
-  val asfs_map_add : Abstract.asfs_map -> nat -> Abstract.asfs_map_val -> Abstract.asfs_map
+  val smap_add : Abstract.smap -> nat -> Abstract.smap_val -> Abstract.smap
 
-  val add_val_asfs : Concrete.opm -> Abstract.asfs -> Abstract.asfs_map_val -> Abstract.asfs option
+  val add_val_asfs :
+    Concrete.stack_op_map -> Abstract.sstate -> Abstract.smap_val ->
+    Abstract.sstate option
 
-  val symbolic_exec'' : Concrete.instr -> Abstract.asfs -> Concrete.opm -> Abstract.asfs option
+  val symbolic_exec'' :
+    Concrete.instr -> Abstract.sstate -> Concrete.stack_op_map ->
+    Abstract.sstate option
 
-  val symbolic_exec' : Concrete.block -> Abstract.asfs -> Concrete.opm -> Abstract.asfs option
+  val symbolic_exec' :
+    Concrete.block -> Abstract.sstate -> Concrete.stack_op_map ->
+    Abstract.sstate option
 
-  val symbolic_exec : Concrete.block -> nat -> Concrete.opm -> Abstract.asfs option
+  val symbolic_exec :
+    Concrete.block -> nat -> Concrete.stack_op_map -> Abstract.sstate option
 
-  val is_comm_op : Concrete.oper_label -> Concrete.opm -> bool
+  val is_comm_op : Concrete.stack_op_instr -> Concrete.stack_op_map -> bool
 
   val apply_f_opt_list : ('a1 -> 'a2 option) -> 'a1 list -> 'a2 list option
 
-  val flat_stack_elem : Abstract.asfs_stack_val -> Abstract.asfs_map -> Abstract.stack_expr option
+  val flat_stack_elem :
+    Abstract.sstack_val -> Abstract.smap -> Abstract.stack_expr option
 
-  val compare_lists_pred : ('a1 -> 'a2 -> bool) -> 'a1 list -> 'a2 list -> bool
+  val compare_lists_pred :
+    ('a1 -> 'a2 -> bool) -> 'a1 list -> 'a2 list -> bool
 
-  val compare_flat_asfs_map_val : Abstract.stack_expr -> Abstract.stack_expr -> Concrete.opm -> bool
+  val compare_flat_smap_val :
+    Abstract.stack_expr -> Abstract.stack_expr -> Concrete.stack_op_map ->
+    bool
 
-  val asfs_eq_stack_elem : Abstract.asfs_stack_val -> Abstract.asfs_stack_val -> Abstract.asfs_map -> Abstract.asfs_map -> Concrete.opm -> bool
+  val asfs_eq_stack_elem :
+    Abstract.sstack_val -> Abstract.sstack_val -> Abstract.smap ->
+    Abstract.smap -> Concrete.stack_op_map -> bool
 
-  val asfs_eq_stack : Abstract.asfs_stack -> Abstract.asfs_stack -> Abstract.asfs_map -> Abstract.asfs_map -> Concrete.opm -> bool
+  val asfs_eq_stack :
+    Abstract.sstack -> Abstract.sstack -> Abstract.smap -> Abstract.smap ->
+    Concrete.stack_op_map -> bool
 
-  val eq_sstate_chkr : Abstract.asfs -> Abstract.asfs -> Concrete.opm -> bool
+  val eq_sstate_chkr :
+    Abstract.sstate -> Abstract.sstate -> Concrete.stack_op_map -> bool
  end
 
 module Coq_Optimizations :
  sig
   val stack_val_is_oper_suffix :
-    Concrete.oper_label -> Abstract.asfs_stack_val -> Abstract.asfs_map -> ((Abstract.asfs_stack_val list * Abstract.asfs_map) * nat) option
+    Concrete.stack_op_instr -> Abstract.sstack_val -> Abstract.smap ->
+    ((Abstract.sstack * Abstract.smap) * nat) option
 
-  val stack_val_is_oper : Concrete.oper_label -> Abstract.asfs_stack_val -> Abstract.asfs_map -> Abstract.asfs_stack_val list option
+  val stack_val_is_oper :
+    Concrete.stack_op_instr -> Abstract.sstack_val -> Abstract.smap ->
+    Abstract.sstack option
 
-  val optimize_fresh_var2 : Abstract.asfs -> Abstract.asfs_map -> (nat -> Abstract.asfs -> Abstract.asfs option) -> Abstract.asfs * bool
+  val optimize_fresh_var2 :
+    Abstract.sstate -> Abstract.smap -> (nat -> Abstract.sstate ->
+    Abstract.sstate option) -> Abstract.sstate * bool
 
-  val optimize_fresh_var : (nat -> Abstract.asfs -> Abstract.asfs option) -> Abstract.asfs -> Abstract.asfs * bool
+  val optimize_fresh_var :
+    (nat -> Abstract.sstate -> Abstract.sstate option) -> Abstract.sstate ->
+    Abstract.sstate * bool
 
-  val stack_val_has_value' : Abstract.asfs_stack_val -> Abstract.asfs_map -> EVM_Def.coq_EVMWord -> bool
+  val stack_val_has_value' :
+    Abstract.sstack_val -> Abstract.smap -> EVM_Def.coq_EVMWord -> bool
 
-  val optimize_func_map : (nat -> Abstract.asfs_map -> Abstract.asfs_map option) -> nat -> Abstract.asfs -> Abstract.asfs option
+  val optimize_func_map :
+    (nat -> Abstract.smap -> Abstract.smap option) -> nat -> Abstract.sstate
+    -> Abstract.sstate option
 
-  val optimize_map_add_zero : nat -> Abstract.asfs_map -> Abstract.asfs_map option
+  val optimize_map_add_zero : nat -> Abstract.smap -> Abstract.smap option
 
-  val optimize_add_zero_fvar : nat -> Abstract.asfs -> Abstract.asfs option
+  val optimize_add_zero_fvar :
+    nat -> Abstract.sstate -> Abstract.sstate option
 
-  val optimize_add_zero : Abstract.asfs -> Abstract.asfs * bool
+  val optimize_add_zero : Abstract.sstate -> Abstract.sstate * bool
 
-  val optimize_map_mul_one : nat -> Abstract.asfs_map -> Abstract.asfs_map option
+  val optimize_map_mul_one : nat -> Abstract.smap -> Abstract.smap option
 
-  val optimize_mul_one_fvar : nat -> Abstract.asfs -> Abstract.asfs option
+  val optimize_mul_one_fvar : nat -> Abstract.sstate -> Abstract.sstate option
 
-  val optimize_mul_one : Abstract.asfs -> Abstract.asfs * bool
+  val optimize_mul_one : Abstract.sstate -> Abstract.sstate * bool
 
-  val optimize_map_mul_zero : nat -> Abstract.asfs_map -> Abstract.asfs_map option
+  val optimize_map_mul_zero : nat -> Abstract.smap -> Abstract.smap option
 
-  val optimize_mul_zero_fvar : nat -> Abstract.asfs -> Abstract.asfs option
+  val optimize_mul_zero_fvar :
+    nat -> Abstract.sstate -> Abstract.sstate option
 
-  val optimize_mul_zero : Abstract.asfs -> Abstract.asfs * bool
+  val optimize_mul_zero : Abstract.sstate -> Abstract.sstate * bool
 
-  val optimize_map_not_not : nat -> Abstract.asfs_map -> Abstract.asfs_map option
+  val optimize_map_not_not : nat -> Abstract.smap -> Abstract.smap option
 
-  val optimize_not_not_fvar : nat -> Abstract.asfs -> Abstract.asfs option
+  val optimize_not_not_fvar : nat -> Abstract.sstate -> Abstract.sstate option
 
-  val optimize_not_not : Abstract.asfs -> Abstract.asfs * bool
+  val optimize_not_not : Abstract.sstate -> Abstract.sstate * bool
 
-  val flat_extract_const : Abstract.asfs_stack_val -> Abstract.asfs_map -> EVM_Def.coq_EVMWord option
+  val flat_extract_const :
+    Abstract.sstack_val -> Abstract.smap -> EVM_Def.coq_EVMWord option
 
-  val const_list : Abstract.asfs_stack_val list -> Abstract.asfs_map -> EVM_Def.coq_EVMWord list option
+  val const_list :
+    Abstract.sstack -> Abstract.smap -> EVM_Def.coq_EVMWord list option
 
-  val optimize_map_eval : Concrete.opm -> nat -> Abstract.asfs_map -> Abstract.asfs_map option
+  val optimize_map_eval :
+    Concrete.stack_op_map -> nat -> Abstract.smap -> Abstract.smap option
 
-  val optimize_eval_fvar : nat -> Abstract.asfs -> Abstract.asfs option
+  val optimize_eval_fvar : nat -> Abstract.sstate -> Abstract.sstate option
 
-  val optimize_eval : Abstract.asfs -> Abstract.asfs * bool
+  val optimize_eval : Abstract.sstate -> Abstract.sstate * bool
 
-  val optimize_map_div_one : nat -> Abstract.asfs_map -> Abstract.asfs_map option
+  val optimize_map_div_one : nat -> Abstract.smap -> Abstract.smap option
 
-  val optimize_div_one_fvar : nat -> Abstract.asfs -> Abstract.asfs option
+  val optimize_div_one_fvar : nat -> Abstract.sstate -> Abstract.sstate option
 
-  val optimize_div_one : Abstract.asfs -> Abstract.asfs * bool
+  val optimize_div_one : Abstract.sstate -> Abstract.sstate * bool
 
-  val optimize_map_eq_zero : nat -> Abstract.asfs_map -> Abstract.asfs_map option
+  val optimize_map_eq_zero : nat -> Abstract.smap -> Abstract.smap option
 
-  val optimize_eq_zero_fvar : nat -> Abstract.asfs -> Abstract.asfs option
+  val optimize_eq_zero_fvar : nat -> Abstract.sstate -> Abstract.sstate option
 
-  val optimize_eq_zero : Abstract.asfs -> Abstract.asfs * bool
+  val optimize_eq_zero : Abstract.sstate -> Abstract.sstate * bool
 
-  val optimize_map_gt_one : nat -> Abstract.asfs_map -> Abstract.asfs_map option
+  val optimize_map_gt_one : nat -> Abstract.smap -> Abstract.smap option
 
-  val optimize_gt_one_fvar : nat -> Abstract.asfs -> Abstract.asfs option
+  val optimize_gt_one_fvar : nat -> Abstract.sstate -> Abstract.sstate option
 
-  val optimize_gt_one : Abstract.asfs -> Abstract.asfs * bool
+  val optimize_gt_one : Abstract.sstate -> Abstract.sstate * bool
 
-  val optimize_map_lt_one : nat -> Abstract.asfs_map -> Abstract.asfs_map option
+  val optimize_map_lt_one : nat -> Abstract.smap -> Abstract.smap option
 
-  val optimize_lt_one_fvar : nat -> Abstract.asfs -> Abstract.asfs option
+  val optimize_lt_one_fvar : nat -> Abstract.sstate -> Abstract.sstate option
 
-  val optimize_lt_one : Abstract.asfs -> Abstract.asfs * bool
+  val optimize_lt_one : Abstract.sstate -> Abstract.sstate * bool
 
-  val optimize_map_or_zero : nat -> Abstract.asfs_map -> Abstract.asfs_map option
+  val optimize_map_or_zero : nat -> Abstract.smap -> Abstract.smap option
 
-  val optimize_or_zero_fvar : nat -> Abstract.asfs -> Abstract.asfs option
+  val optimize_or_zero_fvar : nat -> Abstract.sstate -> Abstract.sstate option
 
-  val optimize_or_zero : Abstract.asfs -> Abstract.asfs * bool
+  val optimize_or_zero : Abstract.sstate -> Abstract.sstate * bool
 
-  val optimize_map_sub_x_x : nat -> Abstract.asfs_map -> Abstract.asfs_map option
+  val optimize_map_sub_x_x : nat -> Abstract.smap -> Abstract.smap option
 
-  val optimize_sub_x_x_fvar : nat -> Abstract.asfs -> Abstract.asfs option
+  val optimize_sub_x_x_fvar : nat -> Abstract.sstate -> Abstract.sstate option
 
-  val optimize_sub_x_x : Abstract.asfs -> Abstract.asfs * bool
+  val optimize_sub_x_x : Abstract.sstate -> Abstract.sstate * bool
 
-  val optimize_map_iszero3 : nat -> Abstract.asfs_map -> Abstract.asfs_map option
+  val optimize_map_iszero3 : nat -> Abstract.smap -> Abstract.smap option
 
-  val optimize_iszero3_fvar : nat -> Abstract.asfs -> Abstract.asfs option
+  val optimize_iszero3_fvar : nat -> Abstract.sstate -> Abstract.sstate option
 
-  val optimize_iszero3 : Abstract.asfs -> Abstract.asfs * bool
+  val optimize_iszero3 : Abstract.sstate -> Abstract.sstate * bool
 
-  val optimize_map_and_and_l : nat -> Abstract.asfs_map -> Abstract.asfs_map option
+  val optimize_map_and_and_l : nat -> Abstract.smap -> Abstract.smap option
 
-  val optimize_and_and_l_fvar : nat -> Abstract.asfs -> Abstract.asfs option
+  val optimize_and_and_l_fvar :
+    nat -> Abstract.sstate -> Abstract.sstate option
 
-  val optimize_and_and_l : Abstract.asfs -> Abstract.asfs * bool
+  val optimize_and_and_l : Abstract.sstate -> Abstract.sstate * bool
 
-  val optimize_map_and_and_r : nat -> Abstract.asfs_map -> Abstract.asfs_map option
+  val optimize_map_and_and_r : nat -> Abstract.smap -> Abstract.smap option
 
-  val optimize_and_and_r_fvar : nat -> Abstract.asfs -> Abstract.asfs option
+  val optimize_and_and_r_fvar :
+    nat -> Abstract.sstate -> Abstract.sstate option
 
-  val optimize_and_and_r : Abstract.asfs -> Abstract.asfs * bool
+  val optimize_and_and_r : Abstract.sstate -> Abstract.sstate * bool
 
-  val apply_n_times : Optimizations.optimization -> nat -> Abstract.asfs -> Abstract.asfs * bool
+  val apply_n_times :
+    Optimizations.optim -> nat -> Abstract.sstate -> Abstract.sstate * bool
 
-  val apply_all_possible_opt : Optimizations.optimization list -> Abstract.asfs -> Abstract.asfs * bool
+  val apply_all_possible_opt :
+    Optimizations.optim list -> Abstract.sstate -> Abstract.sstate * bool
 
-  val apply_pipeline_n_times : Optimizations.optimization list -> nat -> Abstract.asfs -> Abstract.asfs * bool
+  val apply_pipeline_n_times :
+    Optimizations.optim list -> nat -> Abstract.sstate ->
+    Abstract.sstate * bool
 
-  val our_optimization_pipeline : (Abstract.asfs -> Abstract.asfs * bool) list
+  val our_optimization_pipeline :
+    (Abstract.sstate -> Abstract.sstate * bool) list
  end
 
 module Checker :
  sig
   val evm_eq_block_chkr : Concrete.block -> Concrete.block -> nat -> bool
 
-  val evm_eq_block_chkr' : Optimizations.optimization -> Concrete.block -> Concrete.block -> nat -> bool
+  val evm_eq_block_chkr' :
+    Optimizations.optim -> Concrete.block -> Concrete.block -> nat -> bool
 
-  val evm_eq_block_chkr'' : Optimizations.optimization -> Concrete.block -> Concrete.block -> nat -> bool
+  val evm_eq_block_chkr'' :
+    Optimizations.optim -> Concrete.block -> Concrete.block -> nat -> bool
  end
 
 module Parser :
@@ -631,21 +667,24 @@ module Parser :
 
   val parse_non_push_instr : char list -> Concrete.instr option
 
-  val parse_block' : char list list -> Concrete.instr list option
+  val parse_block' : char list list -> Concrete.block option
 
-  val parse_block : char list -> Concrete.instr list option
+  val parse_block : char list -> Concrete.block option
 
-  val opt : Abstract.asfs -> Abstract.asfs * bool
+  val opt : Abstract.sstate -> Abstract.sstate * bool
 
-  val str_to_opt : char list -> Optimizations.optimization option
+  val str_to_opt : char list -> Optimizations.optim option
 
-  val strs_to_opts : char list list -> Optimizations.optimization list option
+  val strs_to_opts : char list list -> Optimizations.optim list option
 
-  val parse_opts : char list list -> Optimizations.optimization option
+  val parse_opts : char list list -> Optimizations.optim option
 
-  val block_eq_0 : char list -> char list -> char list -> Optimizations.optimization -> bool option
+  val block_eq_0 :
+    char list -> char list -> char list -> Optimizations.optim -> bool option
 
-  val block_eq_1 : char list -> char list -> char list -> Optimizations.optimization -> bool option
+  val block_eq_1 :
+    char list -> char list -> char list -> Optimizations.optim -> bool option
 
-  val block_eq_2 : char list -> char list -> char list -> Optimizations.optimization -> bool option
+  val block_eq_2 :
+    char list -> char list -> char list -> Optimizations.optim -> bool option
  end
