ver2/optimizations_def.v
@@ -29,6 +29,8 @@ Import ListNotations.
 Require Import symbolic_state_cmp_impl.
 Import SymbolicStateCmpImp.
 
+Require Import symbolic_state_eval_facts.
+
 Module Optimizations_Def.
 
 Definition optim := sstate -> sstate*bool.
@@ -42,95 +44,108 @@ opt sst = (sst', b) ->
                          eval_sstate st sst' evm_stack_opm = Some st').
 
 (* sb2 preserves all the successful evaluations of sstack_val in sb1 *)
-Definition preserv_sbindings (sb1 sb2: sbindings) : Prop :=
+Definition preserv_sbindings (sb1 sb2: sbindings) (maxidx: nat) 
+  (ops: stack_op_instr_map) : 
+Prop :=
 forall (sv : sstack_val) (stk : stack) (mem: memory) (strg: storage) 
-  (ctx: context) (maxidx: nat) (ops: stack_op_instr_map) (v: EVMWord),
+  (ctx: context) (v: EVMWord),
   eval_sstack_val sv stk mem strg ctx maxidx sb1 ops = Some v ->
   eval_sstack_val sv stk mem strg ctx maxidx sb2 ops = Some v.
   
 (* sb2 preserves all the successful evaluations of sstack in sb1 *)  
 Lemma preserv_sbindings_sstack: 
-forall (sb1 sb2: sbindings), preserv_sbindings sb1 sb2 -> 
+forall (sb1 sb2: sbindings) (maxidx: nat) (ops: stack_op_instr_map), 
+preserv_sbindings sb1 sb2 maxidx ops -> 
   forall (sstk: sstack) (maxid: nat) (stk stk': stack) (mem: memory) 
-    (strg: storage) (ctx: context) (ops: stack_op_instr_map),
+    (strg: storage) (ctx: context),
   eval_sstack sstk maxid sb1 stk mem strg ctx ops = Some stk' ->
   eval_sstack sstk maxid sb2 stk mem strg ctx ops = Some stk'.
 Proof.
 Admitted.
 
+Lemma preserv_sbindings_ext: forall (sb1 sb2: sbindings) 
+  (maxidx: nat) (ops: stack_op_instr_map) (n: nat) (smapv: smap_value),
+preserv_sbindings sb1 sb2 maxidx ops ->
+preserv_sbindings ((n,smapv)::sb1) ((n,smapv)::sb2) maxidx ops.
+Admitted.
+
 (* sb2 preserves all the successful evaluations of smem in sb1 *)  
 Lemma preserv_sbindings_smemory:
-forall (sb1 sb2: sbindings), preserv_sbindings sb1 sb2 -> 
-  forall (smem: smemory) (maxid: nat) (stk: stack) (mem mem': memory) 
-    (strg: storage) (ctx: context) (ops: stack_op_instr_map),
-  eval_smemory smem maxid sb1 stk mem strg ctx ops = Some mem' ->
-  eval_smemory smem maxid sb2 stk mem strg ctx ops = Some mem'.
+forall (sb1 sb2: sbindings) (maxidx: nat) (ops: stack_op_instr_map), 
+preserv_sbindings sb1 sb2 maxidx ops -> 
+  forall (smem: smemory) (stk: stack) (mem mem': memory) 
+    (strg: storage) (ctx: context),
+  eval_smemory smem maxidx sb1 stk mem strg ctx ops = Some mem' ->
+  eval_smemory smem maxidx sb2 stk mem strg ctx ops = Some mem'.
 Proof.
 Admitted.
 
 (* sb2 preserves all the successful evaluations of sstorage in sb1 *)  
 Lemma preserv_sbindings_sstorage:
-forall (sb1 sb2: sbindings), preserv_sbindings sb1 sb2 -> 
-  forall (sstrg: sstorage) (maxid: nat) (stk: stack) (mem: memory) 
-    (strg strg': storage) (ctx: context) (ops: stack_op_instr_map),
-  eval_sstorage sstrg maxid sb1 stk mem strg ctx ops = Some strg' ->
-  eval_sstorage sstrg maxid sb2 stk mem strg ctx ops = Some strg'.
+forall (sb1 sb2: sbindings) (maxidx: nat)
+  (ops: stack_op_instr_map), 
+preserv_sbindings sb1 sb2 maxidx ops -> 
+  forall (stk: stack) (sstrg: sstorage) (mem: memory) (strg strg': storage) (ctx: context),
+  eval_sstorage sstrg maxidx sb1 stk mem strg ctx ops = Some strg' ->
+  eval_sstorage sstrg maxidx sb2 stk mem strg ctx ops = Some strg'.
 Proof.
 Admitted.
 
 
 (* Changing a preseving sbinding in a sstate preserves successful evaluations *)
 Lemma preserv_sbindings_sstate :
-forall (sb1 sb2: sbindings), preserv_sbindings sb1 sb2 ->
+forall (sb1 sb2: sbindings) (maxidx: nat) 
+  (ops: stack_op_instr_map), 
+preserv_sbindings sb1 sb2 maxidx ops ->
   forall (st st': state) (instk_height: nat) (sstk: sstack) (smem: smemory) 
-  (sstrg: sstorage) (sctx : scontext) (ops: stack_op_instr_map) (maxid: nat),
+  (sstrg: sstorage) (sctx : scontext),
     eval_sstate st (SymExState instk_height sstk smem sstrg sctx 
-      (SymMap maxid sb1)) ops = Some st' -> 
+      (SymMap maxidx sb1)) ops = Some st' -> 
     eval_sstate st (SymExState instk_height sstk smem sstrg sctx 
-      (SymMap maxid sb2)) ops = Some st'.
+      (SymMap maxidx sb2)) ops = Some st'.
 Proof.
-intros sb1 sb2 Hpr_sbind st st' instk_height sstk smem sstrg sctx ops maxid
+intros sb1 sb2 maxidx ops Hpr_sbind st st' instk_height sstk smem sstrg sctx
  Heval_sstate_sb1.
 unfold eval_sstate in Heval_sstate_sb1.
 simpl in Heval_sstate_sb1.
 unfold eval_sstate. simpl.
 destruct (instk_height =? length (get_stack_st st)) eqn: eq_instk_height;
   try discriminate.
-destruct (eval_sstack sstk maxid sb1 (get_stack_st st) (get_memory_st st) 
+destruct (eval_sstack sstk maxidx sb1 (get_stack_st st) (get_memory_st st) 
   (get_storage_st st) (get_context_st st) ops) eqn: eq_eval_sstack; 
   try discriminate.
-apply preserv_sbindings_sstack with (sb2:=sb2) in eq_eval_sstack; 
+apply preserv_sbindings_sstack with (sb2:=sb2)(maxidx:=maxidx) in eq_eval_sstack; 
   try assumption.
 rewrite -> eq_eval_sstack.
-destruct (eval_smemory smem maxid sb1 (get_stack_st st) (get_memory_st st)
+destruct (eval_smemory smem maxidx sb1 (get_stack_st st) (get_memory_st st)
   (get_storage_st st) (get_context_st st) ops) eqn: eq_eval_smemory;
   try discriminate.
 apply preserv_sbindings_smemory with (sb2:=sb2) in eq_eval_smemory;
   try assumption.
 rewrite -> eq_eval_smemory.
-destruct (eval_sstorage sstrg maxid sb1 (get_stack_st st) (get_memory_st st)
+destruct (eval_sstorage sstrg maxidx sb1 (get_stack_st st) (get_memory_st st)
   (get_storage_st st) (get_context_st st) ops) eqn: eq_eval_sstorage;
   try discriminate.
 apply preserv_sbindings_sstorage with (sb2:=sb2) in eq_eval_sstorage;
   try assumption.
 rewrite -> eq_eval_sstorage.
-auto.
+intuition.
 Qed.
 
 
 (* Type of a function that optimizes a single smap_value *)
-Definition opt_sbinding_type := sbinding -> sstack_val_cmp -> sbindings -> 
-  nat -> nat -> stack_op_instr_map -> sbinding*bool.
+Definition opt_smap_value_type := smap_value -> sstack_val_cmp -> sbindings -> 
+  nat -> nat -> stack_op_instr_map -> smap_value*bool.
 
  
 (* 'opt' is sound if optimizing the head binding (idx,val) results in a list 
    of sbindings that preserves evaluations *)
-Definition opt_sbinding_snd (opt: opt_sbinding_type) :=
-forall (idx: nat) (val val': smap_value) (fcmp: sstack_val_cmp) (sb: sbindings) 
+Definition opt_sbinding_snd (opt: opt_smap_value_type) :=
+forall (val val': smap_value) (fcmp: sstack_val_cmp) (sb: sbindings) 
   (maxidx: nat) (instk_height: nat) (ops: stack_op_instr_map) (flag: bool),
 sstack_val_cmp_snd fcmp ->
-opt (idx,val) fcmp sb maxidx instk_height ops = ((idx,val'), flag) ->
-  forall stk mem strg ctx v,
+opt val fcmp sb maxidx instk_height ops = (val', flag) ->
+  forall idx stk mem strg ctx v,
   (*instk_height = length stk ->*)
   (*valid_sstack_value instk_height maxidx val ->*)
   (*valid_bindings instk_height maxidx ((idx,val)::sb) ops ->*)
@@ -152,58 +167,80 @@ val = val'.*)
 
 
 (* Applies smap value optimization to the first suitable entry in sbindings *)
-Fixpoint optimize_first_sbindings (opt_sbinding: opt_sbinding_type) 
+Fixpoint optimize_first_sbindings (opt_sbinding: opt_smap_value_type) 
   (fcmp: sstack_val_cmp) (sb: sbindings) (maxid instk_height: nat) 
   (ops: stack_op_instr_map): sbindings*bool :=
 match sb with
 | [] => (sb,false)
 | (n,val)::rs => 
-    match opt_sbinding (n,val) fcmp sb maxid instk_height ops with
-    | (sbind, true) => (sbind::rs, true)
-    | (sbind, false) => 
+    match opt_sbinding val fcmp rs maxid instk_height ops with
+    | (val', true) => ((n,val')::rs, true)
+    | (val', false) => 
         match (optimize_first_sbindings opt_sbinding fcmp rs maxid instk_height ops) with 
-        | (rs', flag) => (sbind::rs', flag)
+        | (rs', flag) => ((n,val)::rs', flag)
         end
     end
 end.
 
+
 (* If opt is sound when optimizing the first entry in the bindings, then 
    the optimize_first_sbindings will preserve the bindings *)
 Lemma opt_sbinding_preserves: 
-forall (opt: opt_sbinding_type) (fcmp: sstack_val_cmp) (sb sb': sbindings) 
+forall (opt: opt_smap_value_type) (fcmp: sstack_val_cmp) (sb sb': sbindings) 
   (maxid instk_height: nat) (ops: stack_op_instr_map) (flag: bool),
+sstack_val_cmp_snd fcmp ->
 opt_sbinding_snd opt ->
 optimize_first_sbindings opt fcmp sb maxid instk_height ops = (sb', flag) ->
-preserv_sbindings sb sb'.
+preserv_sbindings sb sb' maxid ops.
 Proof.
-intros opt fcmp sb sb' maxid instk_height ops flag Hopt_sbinding_snd 
-  Hoptimize_first_sbindings.
-unfold preserv_sbindings. 
-intros sv stk mem strg ctx maxid0 ops0 v Heval_sb.
-destruct sv as [val|var|fvar] eqn: eq_sv.
-- unfold eval_sstack_val in Heval_sb.
-  unfold eval_sstack_val' in Heval_sb.
-  destruct sb as [|h r] eqn: eq_sb.
-  + simpl in Heval_sb.
-    admit.
-  + simpl in Heval_sb.
-    admit.
-- unfold eval_sstack_val in Heval_sb.
-  unfold eval_sstack_val' in Heval_sb.
-  destruct sb as [|h r] eqn: eq_sb.
-  + simpl in Heval_sb.
-    admit.
-  + simpl in Heval_sb.
-    admit.
-- unfold eval_sstack_val in Heval_sb.
-  unfold eval_sstack_val' in Heval_sb.
-  destruct sb as [|h r] eqn: eq_sb.
-  + simpl in Heval_sb. discriminate.
-  + admit. (*simpl in Heval_sb. discriminate.*)
-Admitted.
+intros opt fcmp sb. revert opt fcmp.
+induction sb as [|h rsb IH].
+- intros opt fcmp sb' maxid instk_height ops flag Hfcmp_snd Hopt_sbinding_snd 
+    Hoptimize_first_sbindings.
+  simpl in Hoptimize_first_sbindings.
+  injection Hoptimize_first_sbindings as eq_sb' _.
+  rewrite <- eq_sb'.
+  unfold preserv_sbindings. intuition.
+- intros opt fcmp sb' maxid instk_height ops flag Hfcmp_snd Hopt_sbinding_snd 
+    Hoptimize_first_sbindings.
+  destruct h as [n smapv] eqn: eq_h.
+  unfold optimize_first_sbindings in Hoptimize_first_sbindings.
+  destruct (opt smapv fcmp rsb maxid instk_height ops) as [val' b] 
+    eqn: eq_opt_val.
+  destruct b eqn: eq_b.
+  + (* Optimized first entry in sbindings *)
+    injection Hoptimize_first_sbindings as eq_sb' eq_flag'.
+    rewrite <- eq_sb'.
+    unfold preserv_sbindings.
+    intros sv stk mem strg ctx v Heval_sb.
+    destruct sv as [val|var|fvar] eqn: eq_sv; try intuition.
+    (* FreshVar fvar *)
+    destruct (fvar =? n) eqn: eq_fvar_n.
+    * rewrite -> PeanoNat.Nat.eqb_eq in eq_fvar_n.
+      rewrite -> eq_fvar_n.
+      rewrite -> eq_fvar_n in Heval_sb.
+    unfold opt_sbinding_snd in Hopt_sbinding_snd.
+    pose proof (Hopt_sbinding_snd smapv val' fcmp rsb maxid instk_height ops
+      true Hfcmp_snd eq_opt_val n stk mem strg ctx v) as Hpres_fvar. 
+    apply Hpres_fvar in Heval_sb.
+    assumption.
+    * rewrite -> eval_fvar_diff; try assumption.
+      rewrite -> eval_fvar_diff in Heval_sb; try assumption.
+  + (* Optimized the tail of the sbindings *)
+    fold optimize_first_sbindings in Hoptimize_first_sbindings.
+    destruct (optimize_first_sbindings opt fcmp rsb maxid instk_height ops) as
+      [rs' flag'] eqn: eq_optimize_first_rs.
+    injection Hoptimize_first_sbindings as eq_sb' eq_flag.
+    rewrite <- eq_sb'.
+    pose proof (IH opt fcmp rs' maxid instk_height ops flag' Hfcmp_snd
+      Hopt_sbinding_snd eq_optimize_first_rs) as Hpreserv_rs.
+    apply preserv_sbindings_ext.
+    assumption.
+Qed.
 
 
-Definition optimize_first_sstate (opt: opt_sbinding_type) 
+
+Definition optimize_first_sstate (opt: opt_smap_value_type) 
   (fcmp: sstack_val_cmp) (maxid instk_height: nat) 
   (ops: stack_op_instr_map) (sst: sstate): sstate*bool :=
 match sst with 
@@ -220,23 +257,23 @@ end.
 
 
 
-(* ADD(X,0) or ADD(o,X) = X *)
-Definition optimize_add_0_sbinding : opt_sbinding_type := 
-fun (sbind: sbinding) =>
+(* ADD(X,0) or ADD(0,X) = X *)
+Definition optimize_add_0_sbinding : opt_smap_value_type := 
+fun (val: smap_value) =>
 fun (fcmp: sstack_val_cmp) =>
 fun (sb: sbindings) =>
 fun (maxid: nat) =>
 fun (instk_height: nat) =>
 fun (ops: stack_op_instr_map) => 
-match sbind with
-| (idx, SymOp ADD [arg1; arg2]) => 
+match val with
+| SymOp ADD [arg1; arg2] => 
   if fcmp arg1 (Val WZero) maxid sb maxid sb instk_height ops then
-    ((idx, SymBasicVal arg2), true)
+    (SymBasicVal arg2, true)
   else if fcmp arg2 (Val WZero) maxid sb maxid sb instk_height ops then
-    ((idx, SymBasicVal arg2), true)
+    (SymBasicVal arg2, true)
   else
-    (sbind, false)
-| _ => (sbind, false)
+    (val, false)
+| _ => (val, false)
 end.
 
 Lemma optimize_add_0_sbinding_snd:
